theories/ftlr/Jmp.v
@@ -16,87 +16,100 @@ Section fundamental.
   Implicit Types interp : (D).
 
   Lemma jmp_case (r : leibnizO Reg) (p : Perm)
-        (b e a : Addr) (widc w : Word) (r0 : RegName) (P : D):
-    ftlr_instr r p b e a widc w (Jmp r0) P.
+        (b e a : Addr) (widc w : Word) (src : RegName) (P : D):
+    ftlr_instr r p b e a widc w (Jmp src) P.
   Proof.
     intros Hp Hsome i Hbae Hi.
     iIntros
       "#IH #Hinv_pc #Hinv_idc #Hinva #Hreg #Hread Hown Ha HP Hcls HPC HIDC Hmap".
-    iInsertList "Hmap" [idc;PC].
+    iInsert "Hmap" idc.
 
-    destruct (reg_eq_dec PC r0).
-    * subst r0.
-      iApply (wp_jmp_successPC with "[HPC Ha]"); eauto; first iFrame. 
-      iNext. iIntros "[HPC Ha] /=". 
+    destruct (decide (src = PC)); simplify_map_eq.
+    - iApply (wp_jmp_successPC with "[HPC Ha]"); eauto; first iFrame.
+      iNext. iIntros "[HPC Ha] /=".
       (* reconstruct invariant *)
-      iMod ("Hcls" with "[Ha HP]") as "_";[iExists w;iFrame|]. 
-      iModIntro. 
+      iMod ("Hcls" with "[Ha HP]") as "_";[iExists w;iFrame|].
+      iModIntro.
       iApply wp_pure_step_later; auto.
       (* reconstruct registers *)
-      iNext. 
-      iDestruct ((big_sepM_delete _ _ PC) with "[HPC Hmap]") as "Hmap /=";
-        [apply lookup_insert|rewrite delete_insert_delete;iFrame|]. simpl.
-      (* apply IH *)
-      iIntros "_".
+      iNext. iIntros "_".
+      iInsert "Hmap" PC.
       iApply ("IH" $! _ _ b e a with "[] [] [Hmap] [$Hown]"); eauto.
       { iPureIntro. apply Hsome. }
-      destruct Hp as [-> | ->]; iFrame.
-    * specialize Hsome with r0 as Hr0.
-      destruct Hr0 as [wsrc Hsomesrc].
-      iDestruct ((big_sepM_delete _ _ r0) with "Hmap") as "[Hsrc Hmap]"; eauto.
-      rewrite (lookup_delete_ne r PC r0); eauto.
-      iApply (wp_jmp_success with "[$HPC $Ha $Hsrc]"); eauto.
-      iNext. iIntros "[HPC [Ha Hsrc]] /=".
-      iApply wp_pure_step_later; auto. 
-      (* reconstruct regions *)
-      iDestruct ((big_sepM_delete _ _ r0) with "[Hsrc Hmap]") as "Hmap /=";
-        [apply lookup_insert|rewrite delete_insert_delete;iFrame|]. simpl.
-      rewrite -delete_insert_ne // insert_id; auto.
+      destruct Hp as [-> | ->]; iFrame; by rewrite insert_commute.
 
-      iMod ("Hcls" with "[HP Ha]");[iExists w;iFrame|iModIntro].
+    - destruct (decide (src = idc)); simplify_map_eq.
+      + admit. (* TODO need the wp_rule.... *)
+      + specialize Hsome with src as Hsrc.
+        destruct Hsrc as [wsrc Hsomesrc].
+        iExtractList "Hmap" [src;idc] as ["Hsrc";"Hidc"].
+        iAssert (fixpoint interp1 wsrc) as "#Hinv_src"; first (iApply "Hreg"; eauto).
+        destruct (decide (is_ie_cap wsrc = true)) as [Hie|Hie].
+        * (* EI cap *)
+          destruct wsrc as [ | [ [] b' e' a' | ] | ]; cbn in Hie ; try done; clear Hie.
+          (* open the invariants *)
+          rewrite (fixpoint_interp1_eq (WCap IE _ _ _)) //=.
+          destruct (decide (withinBounds b' e' a' ∧ withinBounds b' e' (a' ^+ 1)%a)) as
+            [Hdec_wb|Hdec_wb].
+          {
+            iDestruct ("Hinv_src" $! Hdec_wb)
+              as (P1 P2) "(Hcond_Pa1 & Hcond_Pa2 & Hinv_a1 & Hinv_a2 & Hexec)";
+              iClear "Hinv_src".
+            (* TODO we can probably encode the disjunction in a better way *)
+            destruct Hdec_wb as [ Hwb%Is_true_true_1 Hwb'%Is_true_true_1].
+            assert (a' ≠ (a' ^+1)%a) by (rewrite withinBounds_true_iff in Hwb'; solve_addr).
+            destruct (decide (a = a')) as [Haeq|Haeq];
+              destruct (decide (a = (a' ^+1)%a)) as [Haeq'|Haeq'].
+            ** (* a' = a , a = a ^+ 1*) solve_addr.
+            ** (* a' = a , a ≠ a ^+ 1*) admit.
+            ** (* a' ≠ a , a = a ^+ 1*) admit.
+            ** (* a' ≠ a , a ≠ a ^+ 1*)
+              iInv "Hinv_a1" as (w1) "[>Ha1 HPa1]" "Hcls_a1".
+              iInv "Hinv_a2" as (w2) "[>Ha2 HPa2]" "Hcls_a2".
 
-     (* Needed because IH disallows non-capability values *)
-      destruct wsrc as [ | [p' b' e' a' | ] | ]; cycle 1.
-      {
-        rewrite /updatePcPerm.
-        (* Special case for E-values*)
-        destruct (decide (p' = E)) as [-> | HneE].
-        -
-          unshelve iDestruct ("Hreg" $! r0 _ _ Hsomesrc) as "HPCv"; auto.
-          iClear "Hinv".
-          rewrite fixpoint_interp1_eq; simpl.
+              iApply (wp_jmp_success_IE with "[$HPC $Hsrc $Hidc $Ha $Ha1 $Ha2]"); eauto.
+              iNext. iIntros "(HPC & Hsrc & Hidc & Ha & Ha1 & Ha2) /=".
+              iApply wp_pure_step_later; auto.
 
-          iDestruct (big_sepM_insert _ _ PC with "[$Hmap $HPC]") as "Hmap"; [apply lookup_delete|]. rewrite insert_delete_insert; auto.
-          iDestruct ("HPCv" with "[$Hmap $Hown]") as "Hcont"; auto.
-        - iAssert (PC ↦ᵣ WCap p' b' e' a')%I  with "[HPC]" as "HPC".
-          { destruct p'; auto. congruence. }
+              iDestruct ("Hcond_Pa1" with "HPa1") as "%Hpers_Pa1".
+              iDestruct ("Hcond_Pa2" with "HPa2") as "%Hpers_Pa2".
+              iDestruct "HPa1" as "#HPa1".
+              iDestruct "HPa2" as "#HPa2".
 
-          iDestruct (big_sepM_insert _ _ PC with "[$Hmap $HPC]") as "Hmap"; [apply lookup_delete|]. rewrite insert_delete_insert; auto.
-          iNext; iIntros "_".
-          iApply ("IH" $! (<[PC:=WCap p' b' e' a']> r) with "[%] [] [Hmap] [$Hown]").
-          { cbn. intros. by repeat (rewrite lookup_insert_is_Some'; right). }
-          { iIntros (ri v Hri Hvs).
-            rewrite lookup_insert_ne in Hvs; auto.
-            destruct (decide (ri = r0)).
-            { subst ri.
-              rewrite Hsomesrc in Hvs; inversion Hvs; subst; clear Hvs.
-              unshelve iSpecialize ("Hreg" $! r0 _ _ Hsomesrc); eauto. }
-            { repeat (rewrite lookup_insert_ne in Hvs); auto.
-              iApply "Hreg"; auto. } }
-          { rewrite insert_insert. iApply "Hmap". }
-          iModIntro.
-          unshelve iSpecialize ("Hreg" $! r0 _ _ Hsomesrc); eauto.
-      }
+              iMod ("Hcls_a2" with "[Ha2 HPa2]") as "_";[iExists w2; iFrame; iFrame "#"|iModIntro].
+              iMod ("Hcls_a1" with "[Ha1 HPa1]") as "_";[iExists w1; iFrame; iFrame "#"|iModIntro].
+              iMod ("Hcls" with "[Ha HP]") as "_";[iExists w; iFrame|iModIntro].
+              iNext ; iIntros "_".
 
-     (* Non-capability cases *)
-      all: iNext; iIntros "_".
-      all: rewrite /updatePcPerm; iApply (wp_bind (fill [SeqCtx]));
-        iApply (wp_notCorrectPC with "HPC"); [intros HFalse; inversion HFalse| ].
-      all: repeat iNext; iIntros "HPC /=".
-      all: iApply wp_pure_step_later; auto.
-      all: iNext; iIntros "_".
-      all: iApply wp_value.
-      all: iIntros; discriminate.
-  Qed.
+              (* Needed because IH disallows non-capability values *)
+              destruct w1 as [ | [p0 b0 e0 a0 | ] | ]; cycle 1.
+              { iApply "Hexec"; iFrame "#"; iFrame.
+                iInsertList "Hmap" [idc;PC].
+                iDestruct (big_sepM_insert _ _ src with "[$Hmap $Hsrc]") as "Hmap".
+                rewrite lookup_insert_ne //= lookup_insert_ne //=.
+                apply lookup_delete; auto.
+                rewrite
+                  (insert_commute _ src) //=
+                    (insert_commute _ src) //=
+                    insert_delete //=
+                    insert_commute //=.
+                iFrame.
+                iIntros (r'). iPureIntro ; apply Hsome.
+              }
+
+              (* Non-capability cases *)
+              all: rewrite /updatePcPerm; iApply (wp_bind (fill [SeqCtx]));
+                iApply (wp_notCorrectPC with "HPC"); [intros HFalse; inversion HFalse| ].
+              all: repeat iNext; iIntros "HPC /=".
+              all: iApply wp_pure_step_later; auto.
+              all: iNext; iIntros "_".
+              all: iApply wp_value.
+              all: iIntros; discriminate.
+          }
+          { (* fail case *)
+            admit.
+          }
+        * (* TODO not EI-cap, works as before *) admit.
+  Admitted.
 
 End fundamental.
